Add compartments to the external call trace events for CminorSel

backend/CminorSel.v
@@ -143,6 +143,7 @@ Inductive state: Type :=
   | Callstate:                          (**r invocation of a fundef  *)
       forall (f: fundef)                (**r fundef to invoke *)
              (args: list val)           (**r arguments provided by caller *)
+             (cp: compartment)          (**r current compartment *)
              (k: cont)                  (**r what to do next  *)
              (m: mem),                  (**r memory state *)
       state
@@ -164,6 +165,7 @@ Section EVAL_EXPR.
 
 Variable sp: val.
 Variable e: env.
+Variable cp: compartment.
 Variable m: mem.
 
 Inductive eval_expr: letenv -> expr -> val -> Prop :=
@@ -192,14 +194,14 @@ Inductive eval_expr: letenv -> expr -> val -> Prop :=
       eval_expr le (Eletvar n) v
   | eval_Ebuiltin: forall le ef al vl v,
       eval_exprlist le al vl ->
-      external_call ef ge vl m E0 v m ->
+      external_call ef ge cp vl m E0 v m ->
       eval_expr le (Ebuiltin ef al) v
   | eval_Eexternal: forall le id sg al b ef vl v,
       Genv.find_symbol ge id = Some b ->
       Genv.find_funct_ptr ge b = Some (External ef) ->
       ef_sig ef = sg ->
       eval_exprlist le al vl ->
-      external_call ef ge vl m E0 v m ->
+      external_call ef ge cp vl m E0 v m ->
       eval_expr le (Eexternal id sg al) v
 
 with eval_exprlist: letenv -> exprlist -> list val -> Prop :=
@@ -348,40 +350,45 @@ Inductive step: state -> trace -> state -> Prop :=
       step (State f Sskip k (Vptr sp Ptrofs.zero) e m)
         E0 (Returnstate Vundef k m')
 
-  | step_assign: forall f id a k sp e m v,
-      eval_expr sp e m nil a v ->
+  | step_assign: forall f cp id a k sp e m v,
+      cp = f.(fn_comp) ->
+      eval_expr sp e cp m nil a v ->
       step (State f (Sassign id a) k sp e m)
         E0 (State f Sskip k sp (PTree.set id v e) m)
 
-  | step_store: forall f chunk addr al b k sp e m vl v vaddr m',
-      eval_exprlist sp e m nil al vl ->
-      eval_expr sp e m nil b v ->
+  | step_store: forall f cp chunk addr al b k sp e m vl v vaddr m',
+      cp = f.(fn_comp) ->
+      eval_exprlist sp e cp m nil al vl ->
+      eval_expr sp e cp m nil b v ->
       eval_addressing ge sp addr vl = Some vaddr ->
       Mem.storev chunk m vaddr v = Some m' ->
       step (State f (Sstore chunk addr al b) k sp e m)
         E0 (State f Sskip k sp e m')
 
-  | step_call: forall f optid sig a bl k sp e m vf vargs fd,
-      eval_expr_or_symbol sp e m nil a vf ->
-      eval_exprlist sp e m nil bl vargs ->
+  | step_call: forall f cp optid sig a bl k sp e m vf vargs fd,
+      cp = f.(fn_comp) ->
+      eval_expr_or_symbol sp e cp m nil a vf ->
+      eval_exprlist sp e cp m nil bl vargs ->
       Genv.find_funct ge vf = Some fd ->
       funsig fd = sig ->
       step (State f (Scall optid sig a bl) k sp e m)
-        E0 (Callstate fd vargs (Kcall optid f sp e k) m)
+        E0 (Callstate fd vargs cp (Kcall optid f sp e k) m)
 
-  | step_tailcall: forall f sig a bl k sp e m vf vargs fd m',
-      eval_expr_or_symbol (Vptr sp Ptrofs.zero) e m nil a vf ->
-      eval_exprlist (Vptr sp Ptrofs.zero) e m nil bl vargs ->
+  | step_tailcall: forall f cp sig a bl k sp e m vf vargs fd m',
+      cp = f.(fn_comp) ->
+      eval_expr_or_symbol (Vptr sp Ptrofs.zero) e cp m nil a vf ->
+      eval_exprlist (Vptr sp Ptrofs.zero) e cp m nil bl vargs ->
       Genv.find_funct ge vf = Some fd ->
       funsig fd = sig ->
       forall COMP: comp_of fd = f.(fn_comp),
       Mem.free m sp 0 f.(fn_stackspace) = Some m' ->
       step (State f (Stailcall sig a bl) k (Vptr sp Ptrofs.zero) e m)
-        E0 (Callstate fd vargs (call_cont k) m')
+        E0 (Callstate fd vargs cp (call_cont k) m')
 
-  | step_builtin: forall f res ef al k sp e m vl t v m',
-      list_forall2 (eval_builtin_arg sp e m) al vl ->
-      external_call ef ge vl m t v m' ->
+  | step_builtin: forall f cp res ef al k sp e m vl t v m',
+      cp = f.(fn_comp) ->
+      list_forall2 (eval_builtin_arg sp e cp m) al vl ->
+      external_call ef ge cp vl m t v m' ->
       step (State f (Sbuiltin res ef al) k sp e m)
          t (State f Sskip k sp (set_builtin_res res v e) m')
 
@@ -389,8 +396,9 @@ Inductive step: state -> trace -> state -> Prop :=
       step (State f (Sseq s1 s2) k sp e m)
         E0 (State f s1 (Kseq s2 k) sp e m)
 
-  | step_ifthenelse: forall f c s1 s2 k sp e m b,
-      eval_condexpr sp e m nil c b ->
+  | step_ifthenelse: forall f cp c s1 s2 k sp e m b,
+      cp = f.(fn_comp) ->
+      eval_condexpr sp e cp m nil c b ->
       step (State f (Sifthenelse c s1 s2) k sp e m)
         E0 (State f (if b then s1 else s2) k sp e m)
 
@@ -412,8 +420,9 @@ Inductive step: state -> trace -> state -> Prop :=
       step (State f (Sexit (S n)) (Kblock k) sp e m)
         E0 (State f (Sexit n) k sp e m)
 
-  | step_switch: forall f a k sp e m n,
-      eval_exitexpr sp e m nil a n ->
+  | step_switch: forall f cp a k sp e m n,
+      cp = f.(fn_comp) ->
+      eval_exitexpr sp e cp m nil a n ->
       step (State f (Sswitch a) k sp e m)
         E0 (State f (Sexit n) k sp e m)
 
@@ -421,8 +430,9 @@ Inductive step: state -> trace -> state -> Prop :=
       Mem.free m sp 0 f.(fn_stackspace) = Some m' ->
       step (State f (Sreturn None) k (Vptr sp Ptrofs.zero) e m)
         E0 (Returnstate Vundef (call_cont k) m')
-  | step_return_1: forall f a k sp e m v m',
-      eval_expr (Vptr sp Ptrofs.zero) e m nil a v ->
+  | step_return_1: forall f cp a k sp e m v m',
+      cp = f.(fn_comp) ->
+      eval_expr (Vptr sp Ptrofs.zero) e cp m nil a v ->
       Mem.free m sp 0 f.(fn_stackspace) = Some m' ->
       step (State f (Sreturn (Some a)) k (Vptr sp Ptrofs.zero) e m)
         E0 (Returnstate v (call_cont k) m')
@@ -436,14 +446,14 @@ Inductive step: state -> trace -> state -> Prop :=
       step (State f (Sgoto lbl) k sp e m)
         E0 (State f s' k' sp e m)
 
-  | step_internal_function: forall f vargs k m m' sp e,
+  | step_internal_function: forall f cp vargs k m m' sp e,
       Mem.alloc m f.(fn_comp) 0 f.(fn_stackspace) = (m', sp) ->
       set_locals f.(fn_vars) (set_params vargs f.(fn_params)) = e ->
-      step (Callstate (Internal f) vargs k m)
+      step (Callstate (Internal f) vargs cp k m)
         E0 (State f f.(fn_body) k (Vptr sp Ptrofs.zero) e m')
-  | step_external_function: forall ef vargs k m t vres m',
-      external_call ef ge vargs m t vres m' ->
-      step (Callstate (External ef) vargs k m)
+  | step_external_function: forall ef cp vargs k m t vres m',
+      external_call ef ge cp vargs m t vres m' ->
+      step (Callstate (External ef) vargs cp k m)
          t (Returnstate vres k m')
 
   | step_return: forall v optid f sp e k m,
@@ -459,7 +469,7 @@ Inductive initial_state (p: program): state -> Prop :=
       Genv.find_symbol ge p.(prog_main) = Some b ->
       Genv.find_funct_ptr ge b = Some f ->
       funsig f = signature_main ->
-      initial_state p (Callstate f nil Kstop m0).
+      initial_state p (Callstate f nil default_compartment Kstop m0).
 
 Inductive final_state: state -> int -> Prop :=
   | final_state_intro: forall r m,
@@ -545,22 +555,22 @@ Proof.
 Qed.
 
 Lemma eval_lift_expr:
-  forall ge sp e m w le a v,
-  eval_expr ge sp e m le a v ->
+  forall ge sp e cp m w le a v,
+  eval_expr ge sp e cp m le a v ->
   forall p le', insert_lenv le p w le' ->
-  eval_expr ge sp e m le' (lift_expr p a) v.
+  eval_expr ge sp e cp m le' (lift_expr p a) v.
 Proof.
   intros until w.
-  apply (eval_expr_ind3 ge sp e m
+  apply (eval_expr_ind3 ge sp e cp m
     (fun le a v =>
       forall p le', insert_lenv le p w le' ->
-      eval_expr ge sp e m le' (lift_expr p a) v)
+      eval_expr ge sp e cp m le' (lift_expr p a) v)
     (fun le al vl =>
       forall p le', insert_lenv le p w le' ->
-      eval_exprlist ge sp e m le' (lift_exprlist p al) vl)
+      eval_exprlist ge sp e cp m le' (lift_exprlist p al) vl)
     (fun le a b =>
       forall p le', insert_lenv le p w le' ->
-      eval_condexpr ge sp e m le' (lift_condexpr p a) b));
+      eval_condexpr ge sp e cp m le' (lift_condexpr p a) b));
   simpl; intros; eauto with evalexpr.
 
   eapply eval_Econdition; eauto. destruct va; eauto.
@@ -576,9 +586,9 @@ Proof.
 Qed.
 
 Lemma eval_lift:
-  forall ge sp e m le a v w,
-  eval_expr ge sp e m le a v ->
-  eval_expr ge sp e m (w::le) (lift a) v.
+  forall ge sp e cp m le a v w,
+  eval_expr ge sp e cp m le a v ->
+  eval_expr ge sp e cp m (w::le) (lift a) v.
 Proof.
   intros. unfold lift. eapply eval_lift_expr.
   eexact H. apply insert_lenv_0.
